label-less substitution (without beta and session)

process/typecheck.v
@@ -9,16 +9,6 @@ From Paco Require Import paco.
 Definition ctxS := list (option sort).
 Definition ctxT := list (option ltt).
 
-Fixpoint onth {A : Type} (n : fin) (lis : list (option A)) : option A :=
-  match lis with 
-    | x::xs =>
-      match n with
-        | S m => onth m xs
-        | 0   => x
-      end
-    | [] => None
-  end.
-
 
 Inductive typ_expr: ctxS -> expr -> sort -> Prop :=
   | sc_var : forall c s t, Some t = onth s c -> typ_expr c (e_var s) t
@@ -42,6 +32,14 @@ Inductive typ_expr: ctxS -> expr -> sort -> Prop :=
                              typ_expr c (e_plus e1 e2) sint.
 
 
+Fixpoint extendLTT (n : fin) (lis : list (option (sort * ltt))) (ST : option (sort * ltt)): list (option (sort * ltt)) :=
+  match n, lis with 
+    | S m, x::xs => x :: extendLTT m xs ST
+    | S m, []    => None :: extendLTT m [] ST
+    | 0,   x::xs => ST :: xs
+    | 0,   []    => ST :: []
+  end.
+ 
 (*  depth *)
 Inductive typ_proc: ctxS -> ctxT -> process -> ltt -> Prop :=
   | tc_inact: forall cs ct,     typ_proc cs ct (p_inact) (ltt_end)
@@ -57,16 +55,14 @@ Inductive typ_proc: ctxS -> ctxT -> process -> ltt -> Prop :=
   | tc_sub  : forall cs ct p t t',    typ_proc cs ct p t ->
                                       subtypeC t t' -> wfC t' ->
                                       typ_proc cs ct p t'
-  | tc_recv : forall cs ct p L ST P T,
-                     length L = length ST ->
-                     length ST = length P ->
-                     length P = length T ->
-                     SSortedNList L ->
-                     Forall2 (fun u v => typ_proc (Some (fst v) :: cs) ct u (snd v)) P (zip ST T) ->
-                     typ_proc cs ct (p_recv p L P) (ltt_recv p (zip L (zip ST T)))
+  | tc_recv : forall cs ct p STT P,
+                     length P = length STT -> SList P ->
+                     Forall2 (fun u v => (u = None /\ v = None) \/ 
+                     (exists p s t, u = Some p /\ v = Some (s, t) /\ typ_proc (Some s :: cs) ct p t)) P STT ->
+                     typ_proc cs ct (p_recv p P) (ltt_recv p STT)
   | tc_send: forall cs ct p l e P S T, typ_expr cs e S ->
                                        typ_proc cs ct P T ->
-                                       typ_proc cs ct (p_send p l e P) (ltt_send p [(l,(S,T))]).
+                                       typ_proc cs ct (p_send p l e P) (ltt_send p (extendLTT l [] (Some (S,T)))).
 
 Print typ_proc_ind.
 
@@ -77,11 +73,11 @@ Section typ_proc_ind_ref.
   Hypothesis P_mu    : forall cs ct p t t', P cs (Some t :: ct) p t' -> subtypeC t t' -> wfC t' -> P cs ct (p_rec p) t'.
   Hypothesis P_ite   : forall cs ct e p1 p2 T, typ_expr cs e sbool -> P cs ct p1 T -> P cs ct p2 T -> P cs ct (p_ite e p1 p2) T.
   Hypothesis P_sub   : forall cs ct p t t', P cs ct p t -> subtypeC t t' -> wfC t' -> P cs ct p t'.
-  Hypothesis P_recv  : forall cs ct p L ST Pr T, length L = length ST -> length ST = length Pr -> length Pr = length T ->
-                     SSortedNList L ->
-                     List.Forall2 (fun u v => P (Some (fst v) :: cs) ct u (snd v)) Pr (zip ST T) ->
-                     P cs ct (p_recv p L Pr) (ltt_recv p (zip L (zip ST T))).
-  Hypothesis P_send  : forall cs ct p l e Pr S T, typ_expr cs e S -> P cs ct Pr T -> P cs ct (p_send p l e Pr) (ltt_send p [(l,(S,T))]).
+  Hypothesis P_recv  : forall cs ct p STT Pr, length Pr = length STT -> SList Pr ->
+                     Forall2 (fun u v => (u = None /\ v = None) \/ 
+                     (exists p s t, u = Some p /\ v = Some (s, t) /\ P (Some s :: cs) ct p t)) Pr STT ->
+                     P cs ct (p_recv p Pr) (ltt_recv p STT).
+  Hypothesis P_send  : forall cs ct p l e Pr S T, typ_expr cs e S -> P cs ct Pr T -> P cs ct (p_send p l e Pr) (ltt_send p (extendLTT l [] (Some (S,T)))).
   
   Fixpoint typ_proc_ind_ref (cs : ctxS) (ct : ctxT) (p : process) (T : ltt) (a : typ_proc cs ct p T) {struct a} : P cs ct p T.
   Proof.
@@ -91,11 +87,14 @@ Section typ_proc_ind_ref.
       | tc_mu sc tc pr t t' Ht Hst Hwf => P_mu sc tc pr t t' (typ_proc_ind_ref sc (Some t :: tc) pr t' Ht) Hst Hwf
       | tc_ite sc tc ex p1 p2 t He Hp1 Hp2 => P_ite sc tc ex p1 p2 t He (typ_proc_ind_ref sc tc p1 t Hp1) (typ_proc_ind_ref sc tc p2 t Hp2)
       | tc_sub sc tc pr t t' Ht Hst Hwf => P_sub sc tc pr t t' (typ_proc_ind_ref sc tc pr t Ht) Hst Hwf
-      | tc_recv sc st p L ST Pr Tr HL HST HP HsL Hm => P_recv sc st p L ST Pr Tr HL HST HP HsL _
+      | tc_recv sc st p STT Pr HST HSl Hm => P_recv sc st p STT Pr HST HSl _
       | tc_send sc tc p l ex Pr Sr Tr He HT => P_send sc tc p l ex Pr Sr Tr He (typ_proc_ind_ref sc tc Pr Tr HT)
     end); try easy.
     revert Hm.
-    apply Forall2_mono. intros. apply (typ_proc_ind_ref (Some (fst y) :: sc) st x (snd y) H).
+    apply Forall2_mono. intros.
+    destruct H. left. easy. destruct H. destruct H. destruct H. right. exists x0, x1, x2.
+    destruct H. destruct H0. split. easy. split. easy.
+    apply typ_proc_ind_ref. easy.
   Qed.
 
 End typ_proc_ind_ref.
@@ -115,83 +114,6 @@ Proof.
     destruct H1.
     easy.
 Qed.
-(* 
-Lemma ref_stronger_C : forall cs cs', refCtxS cs cs' -> leq_ctxS cs cs'. 
-  intros cs cs'.
-  induction 
-  destruct cs, cs'. easy. easy. easy.
-  induction cs. 
-  induction cs'. 
-  easy. easy.
-  intros.
-  
-  
-  induction cs'.
-  
-    
-  induction cs'.
-  easy.
-  intros.
-  simpl in H.
-  simpl in IHcs, IHcs'.
-  
-  
-  unfold refCtxS in *.  
-  
-
-
-Admitted.
-
-Lemma ref_stronger_T : forall ct ct', refCtxT ct ct' -> leq_ctxT ct ct'. 
-Admitted. *)
-
-
-
-(* 
-Lemma ref_ctx_1: forall c c' t t' u,
- refCtxT t t' c c' -> refCtxT u u c c'.
-Proof. intro c.
-       induction c; intros.
-       - case_eq c'; intros.
-         + easy.
-         + subst. simpl in H. easy.
-         + subst. simpl in H. easy.
-       - case_eq c'; intros.
-         + subst. simpl in H. simpl. easy.
-         + subst. simpl. simpl in H.
-           destruct H as (Ha, (Hb, Hc)).
-           subst. split. easy. split. easy.
-           apply IHc with (t := t) (t' := t'). easy.
-         + subst. simpl in H. easy.
-       - case_eq c'; intros.
-         + subst. simpl in H. simpl. easy.
-         + subst. simpl in H. easy.
-         + subst. simpl. simpl in H.
-           destruct H as (Ha, Hb).
-           destruct Ha as [Ha | Ha].
-           destruct Ha as (Ha,(Hc,Hd)).
-           subst.
-           
-           subst. split. easy. split. easy.
-           apply IHc with (t := t) (t' := t'). easy. 
-(*  *)
-Example complex_mu : process := 
-  p_rec (p_recv "Alice" [
-    (0, sbool, p_var 0);
-    (1, sbool, p_rec (p_recv "Bob" [
-       (3, sbool, p_var 0);
-       (4, sbool, p_var 1);
-       (5, sbool, p_inact)
-    ]));
-    (2, sbool, p_inact)
-  ]).
-
-Compute unfold_rec complex_mu. 
- *)
-
-
-
-
 
 
 
