tree/local.v
@@ -1,68 +1,16 @@
 From mathcomp Require Import all_ssreflect.
 From Paco Require Import paco.
 From SST Require Import type.local.
-Require Import List String Datatypes ZArith Relations PeanoNat.
-Local Open Scope list_scope.
+Require Import String List ZArith.
+Local Open Scope string_scope.
 Import ListNotations.
 Require Import Morphisms.
 Require Import Lia.
-Require Import Coq.Init.Datatypes.
-Require Import Coq.Arith.PeanoNat. 
-From mathcomp Require Import ssreflect.seq.
-From Paco Require Import paco.
-
-(* 
-Class nlist (A: Type): Type :=
-{ under: list A;
-  uprop: under <> nil
-}.
-*)
-
-Inductive nlist (A : Type) : Type :=
-  | nnil : A -> nlist A
-  | ncons: A -> nlist A -> nlist A.
-
-Arguments nnil {_} _.
-Arguments ncons {_} _.
-
-Fixpoint nlength {A: Type} (l: nlist A): nat :=
-  match l with
-    | nnil x => S O
-    | ncons x xs => S (nlength xs)
-  end.
-
-Fixpoint nzip {A B: Type} (l1: nlist A) (l2: nlist B): nlist (A*B) :=
-  match (l1, l2) with
-    | (ncons x xs, ncons y ys) => ncons (x,y) (nzip xs ys) 
-    | (nnil x, nnil y)         => nnil (x,y)
-    | (nnil x, ncons y ys)     => nnil (x,y)
-    | (ncons x xs, nnil y)     => nnil (x,y)
-  end. 
-
-Inductive SSortedNList : list fin -> Prop :=
-  | sort1 : forall a, SSortedNList [a]
-  | sort2 : forall (z1 z2 : fin), forall l, le z1 z2 -> SSortedNList (z2 :: l) -> SSortedNList (z1 :: z2 :: l).
-
-Inductive nForall {A : Type} (P : A -> Prop) : nlist A -> Prop :=
-  | nForall_nil:  forall (x : A), P x -> nForall P (nnil x)
-  | nForall_cons : forall (x : A) (l : nlist A), P x -> nForall P l -> nForall P (ncons x l).
-
-Fixpoint nIn {A: Type} (a : A) (l : nlist A): Prop :=
-  match l with
-    | nnil a1     => a = a1
-    | ncons a1 xs => a = a1 \/ nIn a xs
-  end.
-
-(* local session trees *)
-(* CoInductive ltt: Type :=
-  | ltt_end : ltt
-  | ltt_recv: part -> list label -> list sort -> list ltt -> ltt
-  | ltt_send: part -> list label -> list sort -> list ltt -> ltt. *)
 
 CoInductive ltt: Type :=
   | ltt_end : ltt
-  | ltt_recv: part -> list (label*(sort*ltt)) -> ltt
-  | ltt_send: part -> list (label*(sort*ltt)) -> ltt. 
+  | ltt_recv: part -> list (option(sort*ltt)) -> ltt
+  | ltt_send: part -> list (option(sort*ltt)) -> ltt.
 
 Definition ltt_id (s: ltt): ltt :=
   match s with
@@ -71,317 +19,171 @@ Definition ltt_id (s: ltt): ltt :=
     | ltt_send p l => ltt_send p l
   end.
 
-Lemma ltt_eq: forall s, s = ltt_id s.
-Proof. intro s; destruct s; easy. Defined.
-
-Definition nonE {A: Type} (l: list A): Prop :=
-  match l with
-    | [] => False
-    | x::xs => True
+Fixpoint onth {A : Type} (n : fin) (lis : list (option A)) : option A :=
+  match lis with 
+    | x::xs =>
+      match n with
+        | S m => onth m xs
+        | 0   => x
+      end
+    | [] => Datatypes.None
   end.
 
-Definition wfL (l: list fin) := SSortedNList l.
+Fixpoint ozip{A B: Type} (l1: list A) (l2: list B): list (option(A*B)) :=
+  match (l1,l2) with
+    | ([], [])       => []
+    | (x::xs, y::ys) => Datatypes.Some (x, y):: ozip xs ys
+    | _              => [Datatypes.None]
+  end.
 
 Inductive wf (R: ltt -> Prop): ltt -> Prop :=
   | wf_end : wf R ltt_end
-  | wf_recv: forall p l s t,
-             wfL l ->
-             length l = length s ->
-             length s = length t ->
-             Forall R t -> 
-             wf R (ltt_recv p (zip l (zip s t)))
-  | wf_send: forall p l s t,
-             wfL l ->
-             length l = length s ->
-             length s = length t ->
-             Forall R t ->
-             wf R (ltt_send p (zip l (zip s t))).
-
-Lemma mon_wf: monotone1 wf.
-Proof. unfold monotone1.
-       intros.
-       induction IN; intros.
-       - constructor.
-       - constructor. easy. easy. easy.
-         rewrite Forall_forall.
-         intros.
-         apply LE.
-         rewrite Forall_forall in H2.
-         apply H2. easy.
-       - constructor. easy. easy. easy.
-         rewrite Forall_forall.
-         intros.
-         apply LE.
-         rewrite Forall_forall in H2.
-         apply H2. easy.
-Qed.
+  | wf_recv: forall p lis,
+             Forall (fun u => u = Datatypes.None \/ (exists s t, u = Datatypes.Some (s,t) /\ R t)) lis ->
+             wf R (ltt_recv p lis)
+  | wf_send: forall p lis,
+             Forall (fun u => u = Datatypes.None \/ (exists s t, u = Datatypes.Some (s,t) /\ R t)) lis ->
+             wf R (ltt_send p lis).
 
 Definition wfC (t: ltt) := paco1 wf bot1 t.
 
-Class wfltt: Type :=
-{
-   utype: ltt;
-   sprop: wfC utype
-}.
-
-Fixpoint lkp (x: label) (l: list (label*(sort*ltt))): option(sort*ltt) :=
-  match l with
-    | []            => Datatypes.None
-    | (u,(v,t))::xs => if Nat.eqb x u then Datatypes.Some(v,t) else lkp x xs
+Fixpoint wfrec (R1: sort -> sort -> Prop) (R2: ltt -> ltt -> Prop) (l1 l2: list (option(sort*ltt))): Prop :=
+  match (l1,l2) with
+    | (Datatypes.None::xs, Datatypes.None::ys)               => wfrec R1 R2 xs ys
+    | (Datatypes.Some (s,t)::xs, Datatypes.Some (s',t')::ys) => R1 s' s /\ R2 t t' /\ wfrec R1 R2 xs ys
+    | (nil, _)                                               => True
+    | _                                                      => False
   end.
 
-Fixpoint wfrec (R1: sort -> sort -> Prop) (R2: ltt -> ltt -> Prop) (l1 l2: list (label*(sort*ltt))): Prop :=
-  match l1, l2 with
-    | [], _ => True  
-    | ((l,(s,t))::xs), ((l',(s',t'))::ys) => if Nat.eqb l l' then R1 s s' /\ R2 t t' /\ wfrec R1 R2 xs ys
-                                                             else wfrec R1 R2 xs l2 
-    | _, [] => False
-  end.
-
-Fixpoint wfsend (R1: sort -> sort -> Prop) (R2: ltt -> ltt -> Prop) (l1 l2: list (label*(sort*ltt))): Prop :=
-  match l1, l2 with 
-    | _, [] => True  
-    | ((l,(s,t))::xs), ((l',(s',t'))::ys) => if Nat.eqb l l' then R1 s s' /\ R2 t t' /\ wfsend R1 R2 xs ys
-                                                             else wfsend R1 R2 l1 ys 
-    | [], _ => False
-  end.
-
-Fixpoint unzipF {A B C: Type} (l: list(A*(B*C))): list A :=
-  match l with
-    | []            => []
-    | (u,(v,t))::xs => u::unzipF xs 
+Fixpoint wfsend (R1: sort -> sort -> Prop) (R2: ltt -> ltt -> Prop) (l1 l2: list (option(sort*ltt))): Prop :=
+  match (l1,l2) with
+    | (Datatypes.None::xs, Datatypes.None::ys)               => wfsend R1 R2 xs ys
+    | (Datatypes.Some (s',t')::xs, Datatypes.Some (s,t)::ys) => R1 s s' /\ R2 t t' /\ wfsend R1 R2 xs ys
+    | (nil, _)                                               => True
+    | _                                                      => False
   end.
 
 Inductive subtype (R: ltt -> ltt -> Prop): ltt -> ltt -> Prop :=
   | sub_end: subtype R ltt_end ltt_end
   | sub_in : forall p xs ys,
-                    Nat.le (length ys) (length xs) ->
-                    wfrec subsort R xs ys ->
+                    wfrec subsort R ys xs ->
                     subtype R (ltt_recv p xs) (ltt_recv p ys)
   | sub_out : forall p xs ys,
-                     Nat.le (length xs) (length ys) ->
                      wfsend subsort R xs ys ->
                      subtype R (ltt_send p xs) (ltt_send p ys).
 
 Definition subtypeC l1 l2 := paco2 subtype bot2 l1 l2.
 
-Lemma destZip: forall {A B C: Type} (l: list (A * (B * C))),
-               exists L S xs, l = (zip L (zip S xs)).
-Proof. induction l; intros.
-       - exists nil. exists nil. exists nil. easy.
-       - destruct IHl as (L,(S,(xs,Hxs))).
-         destruct a as (a1,(a2,a3)).
-         simpl.
-         exists (a1::L). exists (a2::S). exists(a3::xs).
-         simpl. rewrite Hxs. easy.
-Qed.
-
-Lemma ndestZip: forall {A B C: Type} (l: nlist (A * (B * C))),
-               exists L S xs, l = (nzip L (nzip S xs)).
-Proof. induction l; intros.
-       destruct a as (a1,(a2,a3)).
-       - exists (nnil a1). exists (nnil a2). exists (nnil a3). easy.
-       - destruct IHl as (L,(S,(xs,Hxs))).
-         destruct a as (a1,(a2,a3)).
-         simpl.
-         exists (ncons a1 L). exists (ncons a2 S). exists(ncons a3 xs).
-         simpl. rewrite Hxs. easy.
-Qed.
-
-Lemma unzipIn: forall (l1:  list (label*(sort*ltt))) l s t, In (l, (s, t)) l1 -> In l (unzipF l1).
+Lemma trans_recv: forall (l1 l2 l3:  list (option(sort*ltt))) (R1: sort -> sort -> Prop) (R2: ltt -> ltt -> Prop),
+   Transitive R1 -> Transitive R2 ->
+   wfrec R1 R2 l1 l2 -> wfrec R1 R2 l2 l3 -> wfrec R1 R2 l1 l3.
 Proof. intro l1.
        induction l1; intros.
-       - simpl in *. easy.
-       - simpl in *.
-         destruct H, a, p.
-         inversion H. subst. simpl. left. easy.
-         simpl. right.
-         eapply IHl1. exact H.
+       - simpl. easy.
+       - case_eq l2; case_eq l3; intros.
+         + subst. simpl in *. destruct a. easy.
+         + easy.
+         + subst. simpl in H1. destruct a. destruct p. easy.
+         + easy.
+         + subst. simpl in H2. destruct o. destruct p. easy.
+         + easy.
+         + simpl.
+           destruct a. destruct p, o.
+           destruct p.
+           subst.
+           simpl in H1.
+           destruct o0. destruct p.
+           simpl in H2.
+           split. 
+           transitivity s1. easy. easy.
+           split.
+           transitivity l2. easy. easy.
+           apply IHl1 with (l2 := l0).
+           easy. easy. easy. easy.
+           easy.
+           subst. simpl in *.
+           destruct o0. destruct p. easy.
+           easy.
+           destruct o. subst.
+           simpl in *.
+           destruct o0. destruct p. easy.
+           easy.
+           subst.
+           simpl in *.
+           destruct o0. destruct p. easy.
+           apply IHl1 with (l2 := l0).
+           easy. easy. easy. easy.
 Qed.
 
-Lemma inDiff: forall {A: Type} (l: list A) a b, In a l -> ~In b l -> a <> b.
-Proof. intros A l.
-       induction l; intros.
-       - simpl in H. easy.
-       - simpl in *.
-         intro Ha.
-         destruct H. subst.
-         apply H0. left. easy.
-         subst.
-         apply H0. right. easy. 
-Qed.
-
-Lemma inLkp: forall (l1:  list (label*(sort*ltt))) l s t,
-  NoDup (unzipF l1) ->
-  In (l,(s,t)) l1 <-> lkp l l1 = Datatypes.Some(s, t).
+Lemma trans_send: forall (l1 l2 l3:  list (option(sort*ltt))) (R1: sort -> sort -> Prop) (R2: ltt -> ltt -> Prop),
+   Transitive R1 -> Transitive R2 ->
+   wfsend R1 R2 l1 l2 -> wfsend R1 R2 l2 l3 -> wfsend R1 R2 l1 l3.
 Proof. intro l1.
        induction l1; intros.
-       split.
-       simpl. easy.
-       simpl. easy.
-       split.
-       intro Ha.
-       simpl.
-       destruct a, p.
-       simpl in Ha.
-       destruct Ha. inversion H0. subst.
-       rewrite Nat.eqb_refl. easy.
-       simpl in H.
-       pose proof H0 as H00.
-       apply unzipIn in H0.
-       inversion H. subst.
-       specialize(inDiff _ _ _ H0 H3); intros.
-       assert(Nat.eqb l n = false).
-       { rewrite Nat.eqb_neq. easy. }
-       rewrite H2.
-       apply IHl1. easy. easy.
-       intro Ha.
-       simpl in Ha.
-       destruct a, p. simpl.
-       case_eq(Nat.eqb l n); intros.
-       rewrite H0 in Ha.
-       rewrite Nat.eqb_eq in H0. subst.
-       inversion Ha. subst. left. easy.
-       rewrite H0 in Ha.
-       eapply IHl1 in Ha.
-       right. easy.
-       simpl in H.
-       inversion H. subst. easy.
+       - simpl. easy.
+       - case_eq l2; case_eq l3; intros.
+         + subst. simpl in *. destruct a. easy.
+         + easy.
+         + subst. simpl in H1. destruct a. destruct p. easy.
+         + easy.
+         + subst. simpl in H2. destruct o. destruct p. easy.
+         + easy.
+         + simpl.
+           destruct a. destruct p, o.
+           destruct p.
+           subst.
+           simpl in H1.
+           destruct o0. destruct p.
+           simpl in H2.
+           split. 
+           transitivity s1. easy. easy.
+           split.
+           transitivity l2. easy. easy.
+           apply IHl1 with (l2 := l0).
+           easy. easy. easy. easy.
+           easy.
+           subst. simpl in *.
+           destruct o0. destruct p. easy.
+           easy.
+           destruct o. subst.
+           simpl in *.
+           destruct o0. destruct p. easy.
+           easy.
+           subst.
+           simpl in *.
+           destruct o0. destruct p. easy.
+           apply IHl1 with (l2 := l0).
+           easy. easy. easy. easy.
 Qed.
 
-Lemma ninLkp: forall (l1:  list (label*(sort*ltt))) l,
-  NoDup (unzipF l1) ->
-  (forall s t, (~ In (l,(s,t)) l1)) <-> lkp l l1 = Datatypes.None.
-Proof. intro l1.
-       induction l1; intros.
-       - split. intro Ha.
-         simpl. easy.
-       - intro Ha.
-         simpl. easy.
-       - split. intro Ha.
-         simpl. destruct a, p.
-         simpl in Ha.
-         case_eq(Nat.eqb l n); intros.
-         rewrite Nat.eqb_eq in H0. subst.
-         specialize(Ha s l0).
-         destruct Ha. left. easy.
-         apply IHl1.
-         simpl in H. inversion H. subst. easy.
-         intros.
-         rewrite Nat.eqb_neq in H0.
-         intro Hb.
-         apply H0.
-         specialize(Ha s0 t).
-         destruct Ha. right. easy.
-         
-         intro Ha.
-         intros. simpl in Ha.
-         destruct a, p.
-         case_eq(Nat.eqb l n); intros.
-         rewrite Nat.eqb_eq in H0. subst.
-         rewrite Nat.eqb_refl in Ha.
-         easy.
-         rewrite H0 in Ha.
-         simpl.
-         intro Hb.
-         rewrite Nat.eqb_neq in H0.
-         apply H0.
-         destruct Hb.
-         inversion H1. easy.
-         apply IHl1 in H1. easy.
-         simpl in H. inversion H. easy.
-         easy.
-Qed.
-
-Lemma lkp_eq: forall l1 l2, 
-  NoDup (unzipF l1) ->
-  NoDup (unzipF l2) ->
-  (forall l, lkp l l1 = lkp l l2) <-> (forall x, In x l1 <-> In x l2).
-Proof. intros.
-       split. intros Ha (l,(s,t)).
-       case_eq(lkp l l1); case_eq(lkp l l2); intros.
-       - specialize(Ha l).
-         rewrite inLkp.
-         rewrite inLkp.
-         split.
-         intro Hb. rewrite <- Ha. easy.
-         intro Hb. rewrite Ha. easy.
-         easy. easy.
-         specialize(Ha l).
-         rewrite H1 in Ha.
-         rewrite H2 in Ha.
-         easy.
-         specialize(Ha l).
-         rewrite H1 in Ha.
-         rewrite H2 in Ha.
-         easy.
-         specialize(Ha l).
-         rewrite <- ninLkp in H1.
-         rewrite <- ninLkp in H2.
-         specialize(H1 s t).
-         specialize(H2 s t).
-         split; intro; easy.
-         easy. easy.
-         
-       intros.
-       case_eq(lkp l l1); case_eq(lkp l l2); intros.
-       destruct p, p0.
-       rewrite <- inLkp in H2.
-       rewrite <- inLkp in H3.
-       pose proof H1 as H10.
-       specialize(H1 (l, (s, l0))).
-       specialize(H10 (l, (s0, l3))).
-       apply H10 in H3.
-       rewrite inLkp in H3.
-       rewrite inLkp in H2.
-       rewrite H3 in H2.
-       inversion H2. subst. easy.
-       easy. easy. easy. easy.
-       
-       destruct p.
-       rewrite <- inLkp in H3.
-       rewrite <- ninLkp in H2.
-       specialize(H2 s l0). 
-       apply H1 in H3. easy.
-       easy. easy.
-       destruct p.
-       rewrite <- inLkp in H2.
-       rewrite <- ninLkp in H3.
-       specialize(H3 s l0). 
-       apply H1 in H2. easy.
-       easy. easy.
-       easy.
-Qed.
-
-Lemma refl_recv: forall (l1:  list (label*(sort*ltt))) (R1: sort -> sort -> Prop) (R2: ltt -> ltt -> Prop),
+Lemma refl_recv: forall (l1:  list (option(sort*ltt))) (R1: sort -> sort -> Prop) (R2: ltt -> ltt -> Prop),
    Reflexive R1 -> Reflexive R2 ->
    wfrec R1 R2 l1 l1.
-Proof. intros.
-       induction l1.
-       - easy.
-       - destruct a. destruct p. 
-         simpl.
-         assert ((n =? n)%nat = true). 
-         {
-          induction n. easy. simpl. easy.
-         }
-         replace (n =? n)%nat with true. easy. 
+Proof. intro l1.
+       induction l1; intros.
+       - simpl. easy.
+       - simpl. destruct a. destruct p.
+         split. reflexivity.
+         split. reflexivity.
+         apply IHl1.
+         easy. easy.
+         apply IHl1.
+         easy. easy.
 Qed.
 
-Lemma refl_send: forall (l1:  list (label*(sort*ltt))) (R1: sort -> sort -> Prop) (R2: ltt -> ltt -> Prop),
+Lemma refl_send: forall (l1:  list (option(sort*ltt))) (R1: sort -> sort -> Prop) (R2: ltt -> ltt -> Prop),
    Reflexive R1 -> Reflexive R2 ->
    wfsend R1 R2 l1 l1.
-Proof. intros.
-       induction l1.
-       - easy.
-       - destruct a. destruct p.
-         simpl.
-         assert ((n =? n)%nat = true). 
-         {
-          induction n. easy. simpl. easy.
-         }
-         replace (n =? n)%nat with true.
-         easy.
+Proof. intro l1.
+       induction l1; intros.
+       - simpl. easy.
+       - simpl. destruct a. destruct p.
+         split. reflexivity.
+         split. reflexivity.
+         apply IHl1.
+         easy. easy.
+         apply IHl1.
+         easy. easy.
 Qed.
 
 Lemma stRefl: forall l, subtypeC l l.
@@ -390,259 +192,30 @@ Proof. pcofix CIH.
        pfold.
        case_eq l; intros.
        constructor.
-       constructor. lia.
-       subst.
+       constructor.
        apply refl_recv.
        constructor.
+
        repeat intro.
+       unfold upaco2.
        right. apply CIH.
 
-       constructor. lia.
+       constructor.
        apply refl_send.
        constructor.
        repeat intro.
        right. apply CIH.
 Qed.
 
-Theorem le_Sn_le : forall n m, Nat.le (S n) m -> Nat.le n m.
-Proof.
-  intros n m H. unfold Nat.le in *. 
-  specialize(Nat.le_succ_l n m); intros. destruct H0. clear H1. specialize(H0 H); intros.
-  apply Nat.lt_le_incl; try easy.
-Qed.
+Lemma stTransH: forall l1 l2 l3 R, Transitive R -> subtype R l1 l2 -> subtype R l2 l3 -> subtype R l1 l3.
+Proof. Admitted.
 
+Lemma stTrans: forall l1 l2 l3, subtypeC l1 l2 -> subtypeC l2 l3 -> subtypeC l1 l3.
+Proof. Admitted.
+ 
 
-Lemma trans_recv: forall (l1 l2 l3:  list (label*(sort*ltt))) (R1: sort -> sort -> Prop) (R2: ltt -> ltt -> Prop),
-   Transitive R1 -> Transitive R2 ->
-   Nat.le (length l1) (length l2) ->
-   Nat.le (length l2) (length l3) ->
-   wfrec R1 R2 l1 l2 -> wfrec R1 R2 l2 l3 -> wfrec R1 R2 l1 l3.
-Proof. intros l1.
-       induction l1; intros.
-       - simpl in *.  easy.
-       - destruct a as (l,(s,t)). 
-         destruct l2; try easy. destruct p; try easy. destruct p; try easy.
-         destruct l3; try easy. destruct p; try easy. destruct p; try easy.
-         simpl in *.
-         case_eq (Nat.eqb l n); intros; try easy.
-         - replace (l =? n )%nat with true in H3.
-           case_eq (Nat.eqb n n0)%nat; intros; try easy.
-           - replace (n =? n0)%nat with true in H4.
-             specialize(Nat.eqb_eq l n); intros. destruct H7. clear H8. specialize(H7 H5); intros.
-             specialize(Nat.eqb_eq n n0); intros. destruct H8. clear H9. specialize(H8 H6); intros.
-             specialize(Nat.eqb_eq l n0); intros. destruct H9. clear H9.
-             specialize(eq_trans H7 H8); intros. specialize(H10 H9); intros.
-             replace (l =? n0)%nat with true.
-             destruct H3. destruct H11. destruct H4. destruct H13.
-             pose proof H as T1. pose proof H0 as T2.
-             specialize(H s s0 s1 H3 H4); intros.
-             specialize(H0 t l0 l4 H11 H13); intros.
-             split; try easy. split; try easy. apply IHl1 with (l2 := l2); try easy.
-             specialize(le_S_n (length l1) (length l2) H1); intros. easy.
-             specialize(le_S_n (length l2) (length l3) H2); intros. easy.
-           - replace (n =? n0)%nat with false in H4.
-             specialize(Nat.eqb_eq l n); intros. destruct H7. clear H8. specialize(H7 H5); intros.
-             specialize(Nat.eqb_neq n n0); intros. destruct H8. clear H9. specialize(H8 H6); intros.
-             case_eq (Nat.eqb l n0); intros; try easy.
-             - specialize(Nat.eqb_eq l n0); intros. destruct H10. clear H11. specialize(H10 H9).
-               specialize(eq_trans (esym H7) H10); intros. easy.
-             apply IHl1 with (l2 := l2); intros; try easy.
-             specialize(le_S_n (length l1) (length l2) H1); intros. easy.
-             specialize(le_Sn_le (length l2) ((length l3).+1) H2); intros. easy.
-         - replace (l =? n)%nat with false in H3.
-           - case_eq (Nat.eqb n n0); intros.
-             replace (n =? n0)%nat with true in H4.
-             specialize(Nat.eqb_neq l n); intros. destruct H7. clear H8. specialize(H7 H5); intros.
-             specialize(Nat.eqb_eq n n0); intros. destruct H8. clear H9. specialize(H8 H6); intros.
-             case_eq (Nat.eqb l n0); intros.
-             - specialize(Nat.eqb_eq l n0); intros. destruct H10. clear H11. specialize(H10 H9).
-               specialize(esym (eq_trans H8 (esym H10))); intros. easy.
-             apply IHl1 with (l2 := ((n, (s0, l0)) :: l2)); try easy.
-             apply le_Sn_le; try easy.
-             simpl. replace (n =? n0)%nat with true; try easy.
-           - replace (n =? n0)%nat with false in H4.
-             case_eq (Nat.eqb l n0); intros.
-             - 
-                       
-Admitted.
-
-
-Lemma trans_send: forall (l1 l2 l3:  list (label*(sort*ltt))) (R1: sort -> sort -> Prop) (R2: ltt -> ltt -> Prop),
-   Transitive R1 -> Transitive R2 ->
-   NoDup(unzipF l1) -> NoDup(unzipF l2) -> NoDup(unzipF l3) ->
-   Nat.le (length l1) (length l2) ->
-   Nat.le (length l2) (length l3) ->
-   wfsend R1 R2 l1 l2 -> wfsend R1 R2 l2 l3 -> wfsend R1 R2 l1 l3.
-Proof. intro l1.
-       induction l1; intros.
-       - simpl in H6. 
-Admitted.
-
-Lemma unzipL: forall {A B C: Type} (l1: list A) (l2: list B) (l3: list C),
-  length l1 = length l2 ->
-  length l2 = length l3 ->
-  unzipF (zip l1 (zip l2 l3)) = l1.
-Proof. intros A B C l1.
-       induction l1; intros.
-       - simpl. case_eq l2; case_eq l3; intros.
-         + simpl. easy.
-         + simpl. easy.
-         + simpl. easy.
-         + simpl. easy.
-       - case_eq l2; case_eq l3; intros.
-         + simpl. subst. easy.
-         + simpl. subst. easy.
-         + simpl. subst. easy.
-         + simpl. f_equal.
-           apply IHl1.
-           subst. inversion H. easy.
-           subst. inversion H0. easy.
-Qed.
-
-Lemma reflstH: forall t1 R,
-  Reflexive R ->
-  wfC t1 ->
-  subtype R t1 t1.
-Proof. intros.
-       case_eq t1; intros.
-       constructor.
-       constructor.
-       lia.
-       apply refl_recv.
-       constructor. easy.
-       subst.
-       punfold H0. inversion H0.
-       subst. simpl.
-       unfold wfL in H3.
-(*        rewrite unzipL. easy. easy. easy.
-       apply mon_wf.
-       constructor.
-       lia.
-       apply refl_send.
-       constructor. easy.
-       subst.
-       punfold H0. inversion H0.
-       subst. simpl.
-       unfold wfL in H3.
-       rewrite unzipL. easy. easy. easy.
-       apply mon_wf.
-Qed. *)
-Admitted.
-
-Lemma transtH: forall t1 t2 t3 R,
-  Transitive R ->
-  wfC t1 ->
-  wfC t2 ->
-  wfC t3 ->
-  subtype R t1 t2 ->
-  subtype R t2 t3 ->
-  subtype R t1 t3.
-Proof. intros.
-       case_eq t1; case_eq t2; case_eq t3; intros; try (subst; simpl in *; easy).
-       subst.
-       inversion H3. subst.
-       inversion H4. subst.
-       constructor.
-       lia.
-       apply trans_recv with (l2 := l0).
-       repeat intro.
-       apply sstrans with (s2 := y). easy. easy.
-       easy. 
-       punfold H2.
-       inversion H2. subst.
-       unfold wfL in H7.
-(*        rewrite unzipL. easy. easy. easy.
-       apply mon_wf.
-       punfold H1.
-       inversion H1. subst.
-       unfold wfL in H7.
-       rewrite unzipL. easy. easy. easy.
-       apply mon_wf.
-       punfold H0.
-       inversion H0. subst.
-       unfold wfL in H7.
-       rewrite unzipL. easy. easy. easy.
-       apply mon_wf.
-       lia.
-       lia.
-       easy. easy.
-
-       subst.
-       inversion H3. subst.
-       inversion H4. subst.
-       constructor.
-       lia.
-       apply trans_send with (l2 := l0).
-       repeat intro.
-       apply sstrans with (s2 := y). easy. easy.
-       easy. 
-
-       punfold H0.
-       inversion H0. subst.
-       unfold wfL in H7.
-       rewrite unzipL. easy. easy. easy.
-       apply mon_wf.
-       punfold H1.
-       inversion H1. subst.
-       unfold wfL in H7.
-       rewrite unzipL. easy. easy. easy.
-       apply mon_wf.
-       punfold H2.
-       inversion H2. subst.
-       unfold wfL in H7.
-       rewrite unzipL. easy. easy. easy.
-       apply mon_wf.
-       lia.
-       lia.
-       easy. easy.
-Qed. *)
-Admitted.
-
-Lemma st_mon: monotone2 subtype.
-Proof. unfold monotone2.
-       intros.
-       induction IN; intros.
-       - constructor.
-       - apply sub_in; try easy.
-         revert xs H H0.
-         induction ys; intros. (* easy.
-         destruct a as (l,(s,t)).
-         specialize(helperL ((l,(s,t)) :: ys) xs l s t subsort r); intro HH.
-         pose proof H0 as HN.
-         apply HH in H0.
-         destruct H0 as (s',(t',(Ha,(Hb,Hc)))).
-         simpl.
-         rewrite Hc.
-         split. easy. split. apply LE. easy.
-         apply IHys. simpl in H. lia.
-         simpl in HN. rewrite Hc in HN.
-         easy.
-         lia.
-         simpl. left. easy.
-       - apply sub_out; try easy.
-         revert ys H H0.
-         induction xs; intros. easy.
-         destruct a as (l,(s,t)).
-         specialize(helperR ((l,(s,t)) :: xs) ys l s t subsort r); intro HH.
-         pose proof H0 as HN.
-         apply HH in H0.
-         destruct H0 as (s',(t',(Ha,(Hb,Hc)))).
-         simpl.
-         rewrite Hc.
-         split. easy. split. apply LE. easy.
-         apply IHxs. simpl in H. lia.
-         simpl in HN. rewrite Hc in HN.
-         easy.
-         lia.
-         simpl. left. easy.
-Qed.
- *)
-Admitted.
-
-
-
-#[export]
+(* #[export]
 Declare Instance stTrans: Transitive (subtypeC).
-
+ *)
 (* #[export]
 Declare Instance stRefl: Reflexive (subtypeC). *)
